Setlec/SetR/Weaken.lean
@@ -248,7 +248,7 @@ private theorem wkRedZeta {Δ : List VExpr} {T v b : VExpr} :
   exact .zeta
 
 private theorem wkRedProjRed (hcl : ∀ n ψ, VExpr.Closed (cval n ψ))
-    {Δ : List VExpr} {p P fv ta tta te tte : VExpr}
+    {Δ : List VExpr} {p P fv ta tta te tte TC restC : VExpr}
     {i : Nat} {sn : Name} {entry : ProjEntry} {ci : ConstantInfo}
     {us : List Level} {vs : List VExpr}
     (h1 : env.findProj? sn i = some entry) (h2 : entry.native = true)
@@ -261,7 +261,12 @@ private theorem wkRedProjRed (hcl : ∀ n ψ, VExpr.Closed (cval n ψ))
       (cval entry.ctor
         (Level.substFn φ ci.toConstantVal.levelParams us)) vs)
     (h9 : vs[entry.numParams + i]? = some fv)
+    (hTC : denoteClosed cval env φ
+      (ci.toConstantVal.type.instantiateLevelParams
+        ci.toConstantVal.levelParams us) = some TC)
+    (hTCc : VExpr.Closed TC)
     (_ : Red μ env cval φ Δ p P)
+    (_ : Tele μ env cval φ Δ TC vs restC)
     (_ : Infer μ env cval φ Δ fv ta) (_ : Infer μ env cval φ Δ ta tta)
     (_ : DefEq μ env cval φ Δ tta
       (.sort ((Level.subst entry.levelParams us entry.fieldSort).eval φ)))
@@ -269,6 +274,7 @@ private theorem wkRedProjRed (hcl : ∀ n ψ, VExpr.Closed (cval n ψ))
     (_ : DefEq μ env cval φ Δ tte
       (.sort ((Level.subst entry.levelParams us entry.structSort).eval φ)))
     (ihp : RedW μ env cval φ Δ p P)
+    (ihTele : TeleW μ env cval φ Δ TC vs restC)
     (ihfv : InfW μ env cval φ Δ fv ta)
     (ihta : InfW μ env cval φ Δ ta tta)
     (ihtta : DeqW μ env cval φ Δ tta
@@ -279,12 +285,14 @@ private theorem wkRedProjRed (hcl : ∀ n ψ, VExpr.Closed (cval n ψ))
       (.sort ((Level.subst entry.levelParams us entry.structSort).eval φ))) :
     RedW μ env cval φ Δ (.proj i p) fv := by
   intro n k Δ' H
-  refine Red.projRed (vs := vs.map (·.liftN n k)) h1 h2 h3
-    (by simpa using h4) h5 h6 h7 ?_ ?_ (ihp H) (ihfv H) (ihta H)
-    (ihtta H) (ihP H) (ihte H) (ihtte H)
+  refine Red.projRed (vs := vs.map (·.liftN n k))
+    (restC := restC.liftN n k) h1 h2 h3
+    (by simpa using h4) h5 h6 h7 ?_ ?_ hTC hTCc (ihp H) ?_ (ihfv H)
+    (ihta H) (ihtta H) (ihP H) (ihte H) (ihtte H)
   · rw [h8, liftN_mkAppN, liftN_eq_self_of_closed (hcl _ _)]
   · rw [List.getElem?_map, h9]
     rfl
+  · simpa [liftN_eq_self_of_closed hTCc] using ihTele H
 
 private theorem wkRedStrLit (hcl : ∀ n ψ, VExpr.Closed (cval n ψ))
     {Δ : List VExpr} {s : String} {SC P : VExpr}
